Auto/Lib/IntExtra.lean
@@ -1,0 +1,24 @@
+namespace Auto
+
+-- A version of `Nat.beq_refl` that reduces to `Eq.refl`
+def Nat.beq_refl' : (a : Nat) → (a.beq a) = true
+| 0 => rfl
+| n + 1 => Nat.beq_refl' n
+
+def Int.beq : Int → Int → Bool
+| .ofNat n₁,   .ofNat n₂   => n₁.beq n₂
+| .negSucc n₁, .negSucc n₂ => n₁.beq n₂
+| _,           _           => false
+
+def Int.beq_refl : (i : Int) → (Int.beq i i) = true
+| .ofNat n => Nat.beq_refl' n
+| .negSucc n => Nat.beq_refl' n
+
+def Int.beq_eq (i₁ i₂ : Int) : Int.beq i₁ i₂ → i₁ = i₂ :=
+  match i₁, i₂ with
+  | .ofNat n₁, .ofNat n₂ => fun H => congrArg _ (Nat.eq_of_beq_eq_true H)
+  | .negSucc n₁, .negSucc n₂ => fun H => congrArg _ (Nat.eq_of_beq_eq_true H)
+  | .ofNat n₁, .negSucc n₂ => fun H => by cases H
+  | .negSucc n₁, .ofNat n₂ => fun H => by cases H
+
+end Auto
